ironfleet/ravana/RefinementProof/ControllerLogEvent.dfy
@@ -1,0 +1,132 @@
+include "../Types.i.dfy"
+include "../Refinement.i.dfy"
+include "../Service.i.dfy"
+include "../DistributedSystem.i.dfy"
+include "../RefinementLemmas.i.dfy"
+
+module Refinement_Proof_ControllerLogEvent {
+  import opened Types_i
+  import opened Refinement_i
+  import opened Service_i
+  import opened DistributedSystem_i
+  import opened RefinementLemmas_i
+
+  predicate conditions(rs: RState, rs': RState, p: SwitchIdPair)
+  {
+    rstate_valid(rs)
+
+    && LEnvironment_Next(rs.environment, rs'.environment)
+    && rs.environment.nextStep.LEnvStepHostIos?
+    && rs.endpoint_logger == rs'.endpoint_logger
+    && rs.initControllerState == rs'.initControllerState
+    && rs.environment.nextStep.actor in rs.server_controllers
+    && rs.environment.nextStep.actor in rs'.server_controllers
+    && Node_ControllerLogEvent(
+                rs.server_controllers[rs.environment.nextStep.actor],
+                rs'.server_controllers[rs.environment.nextStep.actor],
+                p,
+                rs.environment.nextStep.ios)
+    && rs.server_switches == rs'.server_switches
+    && rs.server_logger == rs'.server_logger
+    && rs'.server_controllers == rs.server_controllers[
+        rs.environment.nextStep.actor := rs'.server_controllers[rs.environment.nextStep.actor]]
+  }
+
+  lemma lemma_refines_ControllerLogEvent(rs: RState, rs': RState, p: SwitchIdPair)
+  requires conditions(rs, rs', p)
+  ensures rstate_valid(rs')
+  ensures refinement(rs) == refinement(rs')
+  {
+    lemma_packets_are_valid(rs, rs', p);
+
+    lemma_controllers_recved_events_valid_if_recved_events_unchanged(rs, rs');
+
+    assert refinement_switchStates(rs.server_switches)
+        == refinement_switchStates(rs'.server_switches);
+
+    assert refinement_controllerState(rs.server_logger.log, rs.initControllerState)
+        == refinement_controllerState(rs'.server_logger.log, rs'.initControllerState);
+
+    assert refinement_outstandingCommands(rs.server_logger.log, rs.initControllerState, rs.server_switches)
+        == refinement_outstandingCommands(rs'.server_logger.log, rs'.initControllerState, rs'.server_switches);
+
+    assert refinement_outstandingEvents(rs.server_switches, rs.server_logger.log)
+        == refinement_outstandingEvents(rs'.server_switches, rs'.server_logger.log);
+  }
+
+  lemma {:axiom} lemma_packets_are_valid(rs: RState, rs': RState, p: SwitchIdPair)
+  requires conditions(rs, rs', p)
+  ensures packets_are_valid(rs')
+  /*
+  {
+    lemma_new_packet_valid(rs, rs', p);
+    packet_validation_preservation(rs, rs', p);
+    lemma_packets_are_valid_sending_1(rs, rs');
+  }
+  */
+
+  lemma lemma_new_packet_valid(rs: RState, rs': RState, p: SwitchIdPair)
+  requires conditions(rs, rs', p)
+  ensures is_valid_LogMessage(rs', 
+      rs.environment.nextStep.ios[0].s.src,
+      rs.environment.nextStep.ios[0].s.dst,
+      rs.environment.nextStep.ios[0].s.msg)
+  {
+    reveal_controllers_recved_events_valid();
+    assert p.switch in rs.server_switches;
+    assert p.event_id in rs.server_switches[p.switch].bufferedEvents;
+    assert rs.server_switches[p.switch].bufferedEvents[p.event_id] ==
+        rs.server_controllers[rs.environment.nextStep.actor].recved_events[p];
+    var entry := rs.environment.nextStep.ios[0].s.msg.log_entry;
+    assert entry.LMRecv?;
+    assert entry.switch == p.switch;
+    assert entry.switch in rs.server_switches;
+    assert entry.event_id == p.event_id;
+    assert entry.event_id in rs.server_switches[entry.switch].bufferedEvents;
+  }
+
+  lemma packet_validation_preservation(rs: RState, rs': RState, pair: SwitchIdPair)
+  requires conditions(rs, rs', pair)
+  ensures packet_validation_preserved(rs, rs')
+  {
+    forall p : LPacket<EndPoint, RavanaMessage>
+    ensures 
+        is_valid_message(rs, p.src, p.dst, p.msg) ==>
+        is_valid_message(rs', p.src, p.dst, p.msg)
+    {
+      if (is_valid_message(rs, p.src, p.dst, p.msg)) {
+        match p.msg
+          case EventMessage(event: Event, event_id: int) => {
+            assert is_valid_EventMessage(rs', p.src, p.dst, p.msg);
+          }
+          case EventAck(event_ack_id: int) => {
+            assert is_valid_EventAck(rs', p.src, p.dst, p.msg);
+          }
+          case CommandMessage(command: Command, command_id: int) => {
+            assert is_valid_CommandMessage(rs', p.src, p.dst, p.msg);
+          }
+          case CommandAck(command_ack_id: int) => {
+            assert is_valid_CommandAck(rs', p.src, p.dst, p.msg);
+          }
+          case InitNewMaster(leader_id: int) => {
+            assert is_valid_InitNewMaster(rs', p.src, p.dst, p.msg);
+          }
+          case NewMaster(master_id: int) => {
+            assert is_valid_NewMaster(rs', p.src, p.dst, p.msg);
+          }
+          case NewMasterAck => {
+            assert is_valid_NewMasterAck(rs', p.src, p.dst, p.msg);
+          }
+          case LogMessage(log_entry: LogEntry) => {
+            assert is_valid_LogMessage(rs', p.src, p.dst, p.msg);
+          }
+          case LogBroadcastMessage(full_log: seq<LogEntry>) => {
+            assert is_valid_LogBroadcastMessage(rs', p.src, p.dst, p.msg);
+          }
+      }
+    }
+    reveal_packet_validation_preserved();
+  }
+
+
+}
